25/4

Assignment_1.dfy
@@ -10,7 +10,9 @@ class CarPark {
     var generalSpace: set<int>;
 
     // Maximum number of cars in overall 
-    var maxSpots: int;
+    var maxSpace: int;
+
+    var maxReservedSpace: int;
 
     // Set of cars that have a active reservation
     var carsWRes: set<int>;
@@ -20,39 +22,52 @@ class CarPark {
 
 
     // a constructor for the class, setting the car-park up for a new day.
-    constructor (x: int)
+    //x -> size of carpark
+    //y -> size of reservedSpace
+    constructor (x: int, y: int)
+    requires x - 8 > y
+    ensures true;
     {
-        maxSpots := x;
+        maxSpace := x;
+        parkingRestriction := true;
 
     }
 
     // to allow any car without a reservation to enter the car park.
     method enterCarPark (x: int) returns (res: bool)
-    // requires that car does not exist in carparks
-    requires !(x in generalSpace) && !(x in reservedSpace);
-    //ensures that car is either in generalSpace or reservedSpace
-    ensures x in generalSpace || x in reservedSpace
-    //ensures that the collective sum of the two car spaces is 1 larger after the execution
-    ensures |generalSpace|  == old(|generalSpace|) + 1
-    ensures old(reservedSpace) == old(reservedSpace)
+    //ensures that car is either in generalSpace after correct execution
+    ensures res ==> x in generalSpace 
+    //ensures that the sum of the carpark is 1 larger after the method executes correctly
+    ensures res ==> |generalSpace| == old(|generalSpace|) + 1
+    //ensures that the reservedSpace carPark was not touched
+    ensures old(reservedSpace) == reservedSpace
     modifies this;
     {
-        generalSpace := generalSpace + {x};
-        res := true;
+        //check that car does not exist in carparks and if there is free space availalbe
+        if !(x in generalSpace) && !(x in reservedSpace) && |generalSpace| < maxSpace-|reservedSpace|-8 {
+            generalSpace := generalSpace + {x};
+            res := true; 
+        } else {
+            res := false;
+        } 
     }
 
     // to allow any car from any area to leave the car park.
     // x is the id of the car
-    method leaveCarPark(x: int)
-    requires x in generalSpace || x in reservedSpace;
+    method leaveCarPark(x: int) returns (res: bool)
+    requires true;
     // ensures that car is not in the sets anymore
     ensures !(x in generalSpace && x in reservedSpace);
     modifies this;
     {
         if(x in generalSpace) {
             generalSpace := generalSpace - {x};
-        } else {
+            res:= true;
+        } else if (x in reservedSpace) {
             reservedSpace := reservedSpace - {x};
+            res := true;
+        } else {
+            res := false;
         }
     }
 
@@ -62,28 +77,49 @@ class CarPark {
     ensures old(generalSpace) == generalSpace;
     ensures old(reservedSpace) == reservedSpace;
     {
-        res := maxSpots - |generalSpace| - |reservedSpace|;
+        res := maxSpace - |generalSpace| - |reservedSpace| - 8;
     }
     
     // to allow a car with a reservation to enter the car park’s reserved area during its hours of operation, or to enter the car park generally outside these hours.
-    method enterReservedCarPark (x: int) returns (res: int)
-    requires x in carsWRes
-    requires parkingRestriction ==  true
-    ensures old(|reservedSpace|) == |reservedSpace|-1;
-    ensures old(generalSpace) == generalSpace;
+    method enterReservedCarPark (x: int) returns (res: bool)
+    requires true;
+    ensures res ==> old(reservedSpace) + old(generalSpace) + {x} == reservedSpace + generalSpace
+    ensures res ==> old(reservedSpace) == reservedSpace || old(generalSpace) == generalSpace 
     modifies this;
     {
-        reservedSpace :=  reservedSpace + {x};
+        if(x in carsWRes) {
+            if(parkingRestriction) {
+                reservedSpace :=  reservedSpace + {x};
+            } else {
+                generalSpace := generalSpace + {x};
+            }
+            res := true;
+        } else {
+            res := false;
+        }
     }
     
     // to allow a car to be registered as having a reserved space when the owner pays the subscription.
-    method makeSubscription (x: int) returns (res: int)
+    method makeSubscription (x: int) returns (res: bool)
+    requires true;
+    modifies this;
+    ensures old(generalSpace) == generalSpace && old(reservedSpace) == reservedSpace
     {
+        if(!(x in generalSpace || x in reservedSpace) && (|carsWRes| < maxSpace - 8) && !(x in carsWRes)){
+            carsWRes := carsWRes + {x};
+            res := true;
+        } else {
+            res := false;
+        }
 
     }
 
     // to remove parking restrictions on the reserved spaces (i.e. at 3pm).
     method openReservedArea() returns ()
+    ensures old(generalSpace) == generalSpace;
+    ensures old(reservedSpace) == reservedSpace;
+    ensures old(carsWRes) == carsWRes;
+    ensures old(maxSpace) == maxSpace;
     modifies this;
     {
         parkingRestriction := false;
@@ -99,12 +135,94 @@ class CarPark {
         reservedSpace := {};
     }
 
-    // Valid() {
+    predicate Valid()
+    reads this;
+    {
+        maxSpace - 8 - |generalSpace| - |reservedSpace| >= 0
+
+    }
+    method printStats() returns ()
+    requires true
+    ensures old(generalSpace) == generalSpace;
+    ensures old(reservedSpace) == reservedSpace;
+    ensures old(carsWRes) == carsWRes;
+    ensures old(maxSpace) == maxSpace;
+    {
+        var a := generalSpace;
+        var b := reservedSpace;
+        var c := carsWRes;
+        var s := maxSpace;
+
+        print "Free Space", " (", maxSpace - |generalSpace| - |reservedSpace| - 8, ")", "\n";
+
+        while ( s != 0 && 0 < s)
+            decreases s;
+            {
+                print "[ ]", " ";
+                s := s - 1;
+            }
         
-    // }
+        
+
+        print "\n", "\n", "General Space", " (", |generalSpace|, ")", "\n";
+        while ( a != {} )
+        decreases a;
+        {
+            var y :| y in a;
+            print "[", y, "]", " ";
+            a := a - { y };
+        }
+
+        print "\n", "\n", "Reserved Space", " (", |reservedSpace|, ")", "\n";
+        while ( b != {} )
+        decreases b;
+        {
+            var y :| y in b;
+            print "[", y, "]", " ";
+            b := b - { y };
+        }
+
+        print "\n","\n", "Reservations", "\n";
+        while ( c != {} )
+        decreases c;
+        {
+            var y :| y in c;
+            print y, ", ";
+            c := c - { y };
+        }
+    }
 }
 method Main ()  
 {
-    var cp := new CarPark(5);
+    var cp := new CarPark(150, 20);
+    var b1 := cp.makeSubscription(1);
+        
+    //this method call should return false
+    var b2 := cp.makeSubscription(1);
+
+    var b6 := cp.makeSubscription(6);
+
+    var b3 := cp.enterCarPark(2);
+    var b31 := cp.enterCarPark(3);
+    var b311 := cp.leaveCarPark(3);
+    var b32 := cp.enterCarPark(4);
+    var b4 := cp.enterReservedCarPark(1);
     
+    cp.printStats();
+
+    print "\n", "\n", "#### Opening Reserved Area ####", "\n", "\n";
+    cp.openReservedArea();
+
+    var b61 := cp.enterReservedCarPark(6);
+    var b7 := cp.enterCarPark(7);
+
+    // this car has no reservation and should therefore not appear on the general space
+    var b5 := cp.enterReservedCarPark(5);
+    
+    cp.printStats();
+    
+    print "\n", "\n", "#### Closing Car Park ####", "\n", "\n";
+    cp.closeCarPark();
+
+    cp.printStats();
 }
